\documentclass[12pt]{article}

\input{../kz}

\begin{document}
\begin{enumerate}
    \item It suffices to show that any combination $C_1y_1+C_2y_2$ is a solution to the equation.
          If that combination works, then we can plug in $C_1=1$ and $C_2=0$ to see that $y_1$
          is also a solution to the equation and likewise for $y_2$.
          \begin{gather*}
              y=C_1\cos(2t)+C_2\sin(2t) \\
              y'=-2C_1\sin(2t)+2C_2\cos(2t) \\
              y''=-4C_1\cos(2t)-4C_2\sin(2t) \\
              y''+4y=-4C_1\cos(2t)-4C_2\sin(2t)+4C_1\cos(2t)+4C_2\sin(2t)=0
          \end{gather*}
          The provided $y_1$ and $y_2$ do work for the equation.
    \item Like with the previous question, we just have to proave that $C_1y_1+C_2y_2$ works.
          \begin{gather*}
              y=C_1e^{-2t}+C_2te^{-2t}                                \\
              y'=-2C_1e^{-2t}-2C_2te^{-2t}+C_2e^{-2t} \\
              \begin{aligned}
                  y'' & =4C_1e^{-2t}+4C_2te^{-2t}-2C_2e^{-2t}-2C_2e^{-2t} \\
                      & = 4C_1e^{-2t}+4C_2te^{-2t}-4C_2e^{-2t}
              \end{aligned} \\
              4(y+y')=4(-C_1e^{-2t}-C_2te^{-2t}+C_2e^{-2t})=y'' \\
              y''-4y'-4y=0
          \end{gather*}
    \item Let's first verify that $y_1$ and $y_2$ themselves solve the equation.
          \begin{gather*}
              e^t+2e^t-3e^t=0 \\
              9e^{-3t}-6e^{-3t}-3e^{-3t}=0
          \end{gather*}
          We also must prove that their Wronskian is nonzero.
          \begin{align*}
              W(y_1, y_2) & = \det \begin{bmatrix}
                                       e^{-t}  & e^{-3t}   \\
                                       -e^{-t} & -3e^{-3t}
                                   \end{bmatrix} \\
                          & = -3e^{-3t}+e^{-3t}        \\
                          & = -2e^{-3t}                \\
                          & \ne 0
          \end{align*}
          Now that we know we can get a unique solution to any set of ICs with these two equations, we have to solve the set of equations
          \begin{gather*}
              C_1 e^{0} +C_2 e^{-3 \cdot 0} = 1 \\
              C_1(e^{0})+C_2(-3e^{-3 \cdot 0}) = -2
          \end{gather*}
          This reduces to
          \begin{gather*}
              C_1+C_2=1 \\
              C_1-3C_2=-2
          \end{gather*}
          This is trivial to solve and gives us $C_1=\frac{1}{4},C_2=\frac{3}{4} \rightarrow \boxed{y(t)=\frac{1}{4}e^x+\frac{3}{4}e^{-3x}}$. \label{list:3}
    \item We do the same thing as in \ref{list:3}.
          We check that $y_1$ works as a solution:
          \begin{align*}
              y_1'             & =-e^{-t} (2\sin (2t) + \cos (2t))                              \\
              y_1''            & =e^{-t} (4\sin (2t) - 3\cos (2t))                              \\
              y_1''+2y_1'+5y_1 & =e^{-t}(4\sin(2t)-3\cos(2t)-4 \sin (2t)-2 \cos(2t)+5 \cos(2t)) \\
                               & = 0
          \end{align*}
          and do the same for $y_2$:
          \begin{align*}
              y_2'             & =e^{-t}(2 \cos (2t)-\sin (2t))                                     \\
              y_2''            & =-e^{-t}(3 \sin (2t)+4\cos (2t))                                   \\
              y_2''+2y_2'+5y_2 & = e^{-t}(-3 \sin (2t)- 4\cos(2t)+4 \cos(2t)-2 \sin(2t)+5 \sin(2t)) \\
                               & = 0
          \end{align*}
          Then, we compute the Wronskian:
          \begin{align*}
              W(y_1, y_2) & =\det \begin{bmatrix}
                                      e^{-t}\cos(2t)                  & e^{-t}\sin(2t)                  \\
                                      -e^{-t}\cos(2t)-2e^{-t}\sin(2t) & -e^{-t}\sin(2t)+2e^{-t}\cos(2t)
                                  \end{bmatrix}                           \\
                          & = e^{-t}\left(2\cos^2(2t)-\sin(2t)\cos(2t)\right)+e^{-t}\left(2\sin^2(2t)+\sin(2t)\cos(2t)\right) \\
                          & = e^{-t} \left(2\cos^2(2t)+2\sin^2(2t)\right)                                                     \\
                          & = e^{-t} \cdot 2                                                                                  \\
                          & \ne 0
          \end{align*}
          It remains to solve
          \begin{gather*}
              C_1\left(e^{-0}\cos(2 \cdot 0)\right)+C_2\left(e^{-0}\sin(2 \cdot 0)\right)=-1 \\
              C_1\left(-e^{-0}\cos(2 \cdot 0)-2e^{-0}\sin(2 \cdot 0)\right)+C_2\left(-e^{-0}\sin(2 \cdot 0)+2e^{-0}\cos(2 \cdot 0)\right)=0
          \end{gather*}
          This reduces to
          \begin{gather*}
              C_1=-1 \\
              -C_1+2C_2=0
          \end{gather*}
          Thus, we have $C_1=-1$, $C_2=-\frac{1}{2} \rightarrow \boxed{-e^{-t}\cos(2t)-\frac{1}{2}e^{-t}\sin(2t)}$.
    \item This equation is a linear homogeneous differential equation with constant terms.
          In it, $p=0$ and $q=1$, so we have the characteristic equation
          $\lambda^2+0 \cdot \lambda + 1=0$ with the solution $\lambda = \pm i$.
          This gives us the general solution \[y(t)=C_1 \cos t + C_2 \sin t\]
          Solving for the initial condition $y(0)=1$ gives us the final set of solutions \label{list:4}
          \[\boxed{y(t)=\cos t + C_2\sin t}\]
    \item Let's calculate the derivatives of $y_p$ first:
          \begin{gather*}
              y_p'=t(-\sin t)+\cos t \\
              y_p''=-t \cos t - \sin t - \sin t=-t \cos t - 2 \sin t
          \end{gather*}
          Plugging this into the equation, we see that this indeed does solve the given equation:
          \[y_p''+y=-t \cos t - 2 \sin t + t \cos t=-2 \sin t\]
          It remains to solve the homogeneous differential equation
          \[y''+p(t)y'+q(t)y=0\]
          where $p(t)=0$ and $q(t)=1$.
          By our answer in \ref{list:4} and the provided theorem, we have
          \[y(t)=t \cos t + C_1 \cos t + C_2 \sin t\]
          Solving for initial conditions, we have
          \begin{gather*}
              0=C_1 \\
              0=1+C_2
          \end{gather*}
          and so our final solution is
          \[\boxed{y(t)=t \cos t - \sin t}\]
\end{enumerate}
\end{document}
